README.md
@@ -23,7 +23,7 @@ Besides Mathcomp, this also requires the [Equations](https://mattam82.github.io/
 13. [Huffman’s Algorithm](src/huffman.v)
 ### Part III: Priority Queues
 14. [Priority Queues](src/priority.v)
-15. Leftist Heaps
+15. [Leftist Heaps](src/leftist.v)
 16. Priority Queues via Braun Trees
 17. Binomial Heaps
 ### Part IV: Advanced Design and Analysis Techniques
